Update pretty printing of ProofObject.

src/dafny/utils/CFGObject.dfy
@@ -17,10 +17,11 @@ include "../utils/LinSegments.dfy"
 include "../utils/LinSegments.dfy"
 include "../utils/StackElement.dfy"
 include "../utils/Automata.dfy"
+include "../utils/State.dfy"
 include "../utils/CFGState.dfy"
 include "../utils/EVMObject.dfy"
 include "../utils/Statistics.dfy"
-
+include "../prettyprinters/PrettyInstruction.dfy"
 /**
   *  Provides proof objects types.
   */
@@ -29,12 +30,13 @@ module CFGObject {
   import opened MiscTypes
   import opened LinSegments
   import opened Instructions
+  import opened State
   import opened StackElement
   import opened Automata
   import opened CFGState
   import opened EVMObject
   import opened Statistics
-
+  import opened PrettyIns
 
   /**
     *  A CFGObj is a tuple (prog, maxDepth, a, minimised, stats) where:
@@ -54,6 +56,11 @@ module CFGObject {
     ghost predicate IsValid() {
       && |prog.xs| >= 1
       && (forall s:: s in a.states ==> s.IsBounded(|prog.xs|))
+    }
+
+    predicate HasNoErrorState()
+    {
+      prog.HasNoErrorState(a)
     }
 
     /**
@@ -80,14 +87,8 @@ module CFGObject {
         print "*/\n";
       }
 
-      var wPreOperandsCFG := computeWpre();
-
-      if wPreOperandsCFG.Some? {
-        print "// Wpre fixpoint status: ", (if wPreOperandsCFG.v.Left? then "Reached" else "Not reached"), "\n";
-      }
-
       a.ToDot(
-        nodeToString := s requires s in a.states => PrintState(s, noTable, wPreOperandsCFG),
+        nodeToString := s requires s in a.states => prog.ToHTML(s, !noTable, if s.ErrorGState? then None else Some(|s.st|)),
         labelToString := (s, l, _) requires s in a.states && 0 <= l => prog.DotLabel(s, l),
         prefix :=
           "graph[labelloc=\"t\", labeljust=\"l\", label=<"
@@ -100,55 +101,6 @@ module CFGObject {
       } else {
         print "//----------------- Minimised CFG -------------------\n";
       }
-    }
-
-    /**
-      *   Compute the Wpre operands fixpoint of the CFG.
-      */
-    function computeWpre(): (r: Option<Either<seq<nat>, seq<nat>>>)
-      requires this.IsValid()
-      ensures (r.Some? && r.v.Left? ==> |r.v.l| == |a.states|)
-      ensures (r.Some? && r.v.Right? ==> |r.v.r| == |a.states|)
-    {
-      if prog.HasNoErrorState(a) then
-        Some(prog.ComputeWPreOperands(a))
-      else
-        None
-    }
-
-    /**
-      *  Helper to extract the Wpre operands from the result of ComputeWPreOperands.
-      */
-    function ExtractWpre(r: Either<seq<nat>, seq<nat>>): seq<nat>
-    {
-      match r
-      case Left(vv) => vv
-      case Right(vv) => vv
-    }
-
-    /**
-      *  Pretty-print a state.
-      *  @param s        The state to print
-      *  @param noTable  If true, the HTML labels of the nodes are simplified (no tootips, no table).
-      *                  This is useful for large CFGs.
-      *  @param wPre     The Wpre operands mapping for the nodes of the CFG.
-      *              .   If None, the Wpre is not computed and no information about it is printed 
-      *                  in the tooltips.
-      */
-    function PrintState(s: GState, noTable: bool, wPre: Option<Either<seq<nat>, seq<nat>>>): string
-      requires this.IsValid()
-      requires wPre == computeWpre()
-      requires s in a.states
-    {
-      if wPre.Some? then
-        //  the wpre operands is computed and we can print it
-        var wPreValues := ExtractWpre(wPre.v);
-        assert |wPreValues| == |a.states|;
-        //  Because we have a valid CFGObj, we know that the wpre operands are bounded by the number of states
-        //  And as the automaton is valid, indexOf returns a value < |a.states|.
-        prog.ToHTML(s, !noTable, Some(wPreValues[a.indexOf[s]]))
-      else
-        prog.ToHTML(s, !noTable, None)
     }
 
     /**
@@ -172,7 +124,161 @@ module CFGObject {
       + Int.NatToString(numNodes) + " nodes/"
       + Int.NatToString(numEdges) + " edges<BR ALIGN=\"left\"/>"
     }
+
+    /**
+      * Print the CFG object to Dafny.
+      */
+    method {:print} ToDafny(name: string := "EVMProofObject", pathToEVMDafny: string := "")
+      requires this.IsValid()
+      requires this.HasNoErrorState()
+    {
+      //    optional include of the dafny-EVM files
+      if |pathToEVMDafny| > 0 {
+        print "include \"", pathToEVMDafny, "/src/dafny/state.dfy\"", "\n";
+        print "include \"", pathToEVMDafny, "/src/dafny/bytecode.dfy\"", "\n";
+        print "\n";
+      }
+
+      print "include \"./ExternalCallsLib.dfy\"", "\n";
+
+      //    Module
+      print "module " + name + " {", "\n\n";
+      print "import opened Int", "\n";
+      print "import EvmState", "\n";
+      print "import opened Bytecode", "\n";
+      print "import ExternalCallLib", "\n";
+
+      //  build a const with the jumpdests
+      var j := Map(prog.jumpDests, k => "0x" + Hex.NatToHex(k) + ",");
+      /** Set of jumdests. */
+      var jAsString := if |j| == 0 then "{}" else "{" + Init(Flatten(j)) + "}";
+      print "/** Set of valid JUMPDESTS for this program. */", "\n";
+      print "const VALID_JUMPDESTS: set<u256> := " + jAsString + "\n";
+      print "\n";
+      print "/** Lemma for Jumpdest */", "\n";
+      print "lemma {:axiom} ValidJumpDest(s: EvmState.ExecutingState)", "\n";
+      print "   ensures forall k:: k in VALID_JUMPDESTS ==> s.IsJumpDest(k)", "\n";
+
+      // Print the transfer functions for each state of the graph.
+      PrintProofObjectBody();
+      print "}", "\n";
+    }
+
+    /**
+      * Iterate over the states of the CFG and print the transfer functions.
+      */
+    method PrintProofObjectBody(index: nat := 0)
+      requires this.IsValid()
+      requires this.HasNoErrorState()
+      requires index <= |a.states|
+      decreases |a.states| - index
+    {
+      if index < |a.states| {
+        // 
+        var currentState := a.states[index];
+        var startAddress := prog.StartAddress(currentState.segNum);
+        print "\n/** Node " , index , "\n";
+        print "* Segment Id for this node is: ", currentState.segNum, "\n";
+        print "* Starting at 0x", Hex.NatToHex(startAddress),  "\n";
+        print "* Segment type is: ", prog.xs[currentState.segNum].SegTypeName(), "\n";
+        print "* Minimum stack size for this segment to prevent stack underflow: ", prog.WpOp(currentState.segNum), "\n";
+        var minCap := prog.WpCap(currentState.segNum);
+        print "* Minimum capacity for this segment to prevent stack overflow: ", minCap, "\n";
+        var netStackEffect := prog.StackEffect(currentState.segNum);
+        print "* Net Stack Effect: ", (if netStackEffect >= 0 then "+" else "-"), netStackEffect , "\n";
+        var netCapEffect := prog.CapEffect(currentState.segNum);
+        print "* Net Capacity Effect: ", (if netCapEffect >= 0 then "+" else "-"), netStackEffect , "\n";
+        print "*/\n";
+        print "function {:opaque} {:verify false} ExecuteFromCFGNode_s", index, "(s0: EvmState.ExecutingState, gas: nat): (s': EvmState.State)\n";
+        print "  // Writes permission for this segment.", "\n";
+        print "  requires s0.WritesPermitted()", "\n";
+        print "  // PC requirement for this node.", "\n";
+        print "  requires s0.PC() == 0x",  Hex.NatToHex(startAddress), " as nat\n";
+
+        //  requirements on the content of the stack at this node
+        print "  // Stack requirements for this node.", "\n";
+        print "  requires s0.Operands() == ", |currentState.st|, "\n";
+        print "  requires s0.Capacity() >= ", minCap, "\n";
+        for k := 0 to |currentState.st| {
+          if currentState.st[k].Value? {
+            print "\n  requires s0.Peek(", k, ") == ", "0x" + Hex.NatToHex(currentState.st[k].Extract() as nat), "\n";
+          }
+        }
+        print "\n";
+        print "   decreases gas\n";
+
+        //  Print the code for this segment
+        var nodeInstructions := prog.xs[currentState.segNum].ins;
+        print "{\n";
+        print "if gas == 0 then Revert(s0)", "\n";
+        print "else\n";
+        // print "  ValidJumpDest(s0);\n";
+        PrintInstructionsToDafny(nodeInstructions, EState(startAddress, currentState.st));
+        // print "  ValidJumpDest(s", |nodeInstructions|, ");\n";
+        print "  assume s", |nodeInstructions|, ".EXECUTING?", ";\n";
+        print "  assume s", |nodeInstructions|, ".IsJumpDest(s", |nodeInstructions|, ".Peek(0)", ");\n";
+        print "   ", PrintInstructionToDafny(prog.xs[currentState.segNum].lastIns, |nodeInstructions|, |nodeInstructions| + 1), "\n";
+
+        // TODO: assert |a.SuccNat(index)| <= 2;
+        //  Pretty-print the last state.
+        if  |a.SuccNat(index)| == 0 {
+          //    the last state is the state returned.
+          print "  s", |nodeInstructions| + 1, "\n";
+        }
+        else if |a.SuccNat(index)| == 1 {
+          //    this is either a JUMP or a Next but there is unique successor.
+          print "  // jump to the successor Next() or Tgt of JUMP;\n";
+          //   print "  assert ExecuteFromCFGNode_s", a.SuccNat(index)[0], ".requires(s", |nodeInstructions|, ");\n";
+          //   print "s", |nodeInstructions|, "\n";
+
+          print "  ExecuteFromCFGNode_s", a.SuccNat(index)[0], "(s", |nodeInstructions| + 1, ", gas - 1)\n";
+
+        } else {
+          // This must must be two and a JUMPI
+          print "  if s", |nodeInstructions|, ".Peek(1) > 0 then ";
+          //   print "\nassert ExecuteFromCFGNode_s", a.SuccNat(index)[1], ".requires(s", |nodeInstructions|, ");\n";
+          //   print "s", |nodeInstructions|, "\n";
+          print "\nExecuteFromCFGNode_s", a.SuccNat(index)[1], "(s", |nodeInstructions| + 1, ", gas - 1)\n";
+
+          //   print "  else assert ExecuteFromCFGNode_s", a.SuccNat(index)[0], ".requires(s", |nodeInstructions|, ")", ";\n";
+          //   print "s", |nodeInstructions|, "\n";
+          print "  else", "\n";
+          print "     ExecuteFromCFGNode_s", a.SuccNat(index)[0], "(s", |nodeInstructions| + 1, ", gas - 1)", "\n";
+        }
+        print "}\n";
+
+        PrintProofObjectBody(index + 1);
+
+      }
+    }
+
+    /**
+      *   Print out a sequence of instructions in the Dafny-EVM format.
+      */
+    method PrintInstructionsToDafny(xs:seq<ValidInstruction>, currentState: AState, pos: nat := 0)
+    {
+      if |xs| > 0 {
+        var k := PrintInstructionToDafny(xs[0], pos, pos + 1);
+        print "  ", k, "\n";
+        // var newState := currentState;
+        var newState :=
+          if currentState.EState? then
+            xs[0].NextState(currentState, prog.jumpDests, 0)
+          else
+            currentState;
+        if newState.EState? && pos % 3 == 0 {
+          for j := 0 to |newState.stack| {
+            if newState.stack[j].Value?  {
+              print "   assert s", pos + 1, ".Peek(", j, ") == ", "0x" + Hex.NatToHex(newState.stack[j].Extract() as nat), ";\n";
+            }
+          }
+        }
+        PrintInstructionsToDafny(xs[1..], newState, pos + 1);
+      }
+    }
+
   }
+
 
 }
 
